# baseURI: http://www.linked2safety.eu/lmds2

@prefix :        <http://www.linked2safety.eu/lmds2#> .
@prefix acl:     <http://www.w3.org/ns/auth/acl#> .
@prefix dc:      <http://purl.org/dc/elements/1.1/> .
@prefix foaf:    <http://xmlns.com/foaf/0.1/> .
@prefix ont:     <http://www.w3.org/2006/gen/ont#> .
@prefix owl:     <http://www.w3.org/2002/07/owl#> .
@prefix rdf:     <http://www.w3.org/1999/02/22-rdf-syntax-ns#> .
@prefix rdfg-1:  <http://www.w3.org/2004/03/trix/rdfg-1/> .
@prefix rdfs:    <http://www.w3.org/2000/01/rdf-schema#> .
@prefix xsd:     <http://www.w3.org/2001/XMLSchema#> .

@prefix l2s-dim: <http://www.linked2safety-project.eu/dimension/>.

dc:title
      rdf:type owl:AnnotationProperty .

<http://www.linked2safety.eu/lmds2>
      rdf:type owl:Ontology ;
      dc:title "LMDS Security Model (Policy Model)"^^xsd:string ;
      owl:versionInfo "Created with TopBraid Composer"^^xsd:string .

:AccessPolicy
      rdf:type owl:Class ;
      rdfs:subClassOf owl:Thing .

:AccessPolicy1
      rdf:type owl:NamedIndividual , :AccessPolicy ;
      rdfs:comment "An access policy enforced to datacube-graph-2 authorizing only users that their role is defined as 'ClinicalTrialCordinator'"^^xsd:string ;
      :appliesToNamedGraph
              :NamedGraph_14 ;
      :grantsAccess acl:Read_l2s ;
      :hasCondition :Condition7 ;
      :hasUserProfile :UserProfile_4 .

:AccessPolicy10
      rdf:type owl:NamedIndividual , :AccessPolicy ;
      rdfs:comment "An access policy enforced to RDF data-cubes having as dimension the gender and coming from a study project created in clinical sites located in Greece authorizing only users that their role is defined as 'ClinicalTrialCordinator'"^^xsd:string ;
      :grantsAccess acl:Read_l2s ;
      :hasCondition :Condition10 , :Condition9 ;
      :hasUserProfile :UserProfile_4 .

:AccessPolicy2
      rdf:type owl:NamedIndividual , :AccessPolicy ;
      rdfs:comment "An access policy enforced to RDF data-cubes having as dimension dyslipidemia authorizing end-users working in ZEINCRO"^^xsd:string ;
      :grantsAccess acl:Read_l2s ;
      :hasCondition :Condition1 ;
      :hasUserProfile :UserProfile_1 .

:AccessPolicy3
      rdf:type owl:NamedIndividual , :AccessPolicy ;
      rdfs:comment "An access policy enforced to RDF data-cubes having as measure the number of diabetes incidences authorizing only John Smith"^^xsd:string ;
      :grantsAccess acl:Read_l2s ;
      :hasCondition :Condition2 ;
      :hasUser :JohnSmith .

:AccessPolicy4
      rdf:type owl:NamedIndividual , :AccessPolicy ;
      rdfs:comment "An access policy enforced to RDF data-cubes having as dimension drug and dimension values include aspirin and authorizing access to users working in the area of oncology"^^xsd:string ;
      :grantsAccess acl:Read_l2s ;
      :hasCondition :Condition3 ;
      :hasUserProfile :UserProfile_3 .

:AccessPolicy5
      rdf:type owl:NamedIndividual , :AccessPolicy ;
      rdfs:comment "An access policy enforced to RDF data-cubes having as measure occurrence of cancer and measure values is more than 60 (exceeds 60 for at least one observation) authorizing access to users working in the area of oncology and coming from Cyprus"^^xsd:string ;
      :grantsAccess acl:Read_l2s ;
      :hasCondition :Condition4 ;
      :hasUserProfile :UserProfile_3 .

:AccessPolicy6
      rdf:type owl:NamedIndividual , :AccessPolicy ;
      rdfs:comment "An access policy enforced to RDF data-cubes provided by John Smith authorizing end-users working in ZEINCRO"^^xsd:string ;
      :grantsAccess acl:Read_l2s ;
      :hasCondition :Condition5 ;
      :hasUserProfile :UserProfile_1 .

:AccessPolicy7
      rdf:type owl:NamedIndividual , :AccessPolicy ;
      rdfs:comment "An access policy enforced to RDF data-cubes coming from a study project related to lung cancer authorizing only Maria Smith"^^xsd:string ;
      :grantsAccess acl:Read_l2s ;
      :hasCondition :Condition6 ;
      :hasUser :MarySmith .

:AccessPolicy8
      rdf:type owl:NamedIndividual , :AccessPolicy ;
      rdfs:comment "An access policy enforced to RDF data-cubes having as sponsor the \"Xpharma\" authorizing only users that their role is defined as 'ClinicalTrialCordinator'"^^xsd:string ;
      :grantsAccess acl:Read_l2s ;
      :hasCondition :Condition7 ;
      :hasUserProfile :UserProfile_4 .

:AccessPolicy9
      rdf:type owl:NamedIndividual , :AccessPolicy ;
      rdfs:comment "An access policy enforced to RDF data-cubes coming from a study project created in clinical sites located in Greece authorizing only users working in the area of oncology and coming from Cyprus"^^xsd:string ;
      :grantsAccess acl:Read_l2s ;
      :hasCondition :Condition7 ;
      :appliesToNamedGraph
              :NamedGraph_11 ;	  
      :hasUserProfile :UserProfile_3 .

:AccessPolicy_11
      rdf:type :AccessPolicy ;
      :appliesToNamedGraph
              :NamedGraph_11 ;
      :grantsAccess acl:Read_l2s ;
      :hasUser :JohnSmith .

:AccessPolicy_12
      rdf:type :AccessPolicy ;
      :appliesToNamedGraph
              :NamedGraph_12 ;
      :grantsAccess acl:Read_l2s ;
      :hasUser :MarySmith .

:AccessPolicy_13
      rdf:type :AccessPolicy ;
      :appliesToNamedGraph
              :NamedGraph_13 ;
      :grantsAccess acl:Read_l2s ;
      :hasUser :JohnSmith .

:AccessPolicy_14
      rdf:type :AccessPolicy ;
      :appliesToNamedGraph
              :NamedGraph_14 ;
      :grantsAccess acl:Read_l2s ;
      :hasUser :MarySmith .

:AccessPolicy_15
      rdf:type :AccessPolicy ;
      :appliesToNamedGraph
              :NamedGraph_15 ;
      :grantsAccess acl:Read_l2s ;
      :hasUser :JohnSmith , :MarySmith .

:AccessPolicy_16
      rdf:type :AccessPolicy ;
      :appliesToNamedGraph
              :NamedGraph_16 ;
      :grantsAccess acl:Read_l2s ;
      :hasUser :JohnSmith , :MarySmith .

:AccessPolicy_17
      rdf:type :AccessPolicy ;
      :appliesToNamedGraph
              :NamedGraph_17 ;
      :grantsAccess acl:Read_l2s ;
      :hasUser :MarySmith .

:AccessPolicy_18
      rdf:type :AccessPolicy ;
      :appliesToNamedGraph
              :NamedGraph_18 ;
      :grantsAccess acl:Read_l2s ;
      :hasUser :JohnSmith .

:AccessPolicy_19
      rdf:type :AccessPolicy ;
      :appliesToNamedGraph
              :NamedGraph_19 ;
      :grantsAccess acl:Read_l2s ;
      :hasUser :JohnSmith .

:AccessPolicy_20
      rdf:type :AccessPolicy ;
      :appliesToNamedGraph
              :NamedGraph_20 ;
      :grantsAccess acl:Read_l2s ;
      :hasUser :MarySmith .

:AccessPolicy_21
      rdf:type :AccessPolicy ;
      :appliesToNamedGraph
              :NamedGraph_21 ;
      :grantsAccess acl:Read_l2s ;
      :hasUser :JohnSmith , :MarySmith .

:CancerOccurrence
      rdf:type owl:NamedIndividual , :Measure ;
      :hasMinMeasureValue 60 .

:ClinicalResearcher
      rdf:type owl:NamedIndividual , :Role .

:ClinicalTrialCoordinator
      rdf:type owl:NamedIndividual , :Role .

:Condition
      rdf:type owl:Class ;
      rdfs:subClassOf owl:Thing .

:Condition1
      rdf:type owl:NamedIndividual , :Condition ;
      rdfs:comment "Dyslipidemia is one of the dimension of the cube" ;
      :hasDimension l2s-dim:Dyslipidemia .

:Condition10
      rdf:type owl:NamedIndividual , :Condition ;
      rdfs:comment "The project study is located in Cyprus"^^xsd:string ;
      :hasSPLocation "Cyprus"^^xsd:string .

:Condition2
      rdf:type owl:NamedIndividual , :Condition ;
      rdfs:comment "The measure of the data-cube is the diabetes incidences"^^xsd:string ;
      :hasMeasure :DiabetesIncidences .

:Condition3
      rdf:type owl:NamedIndividual , :Condition ;
      rdfs:comment "Aspirin is one of the values receiving the dimension Drug"^^xsd:string ;
      :hasDimension l2s-dim:Drug .

:Condition4
      rdf:type owl:NamedIndividual , :Condition ;
      rdfs:comment "The occurrence of cancer is more than 60"^^xsd:string ;
      :hasMeasure :CancerOccurrence .

:Condition5
      rdf:type owl:NamedIndividual , :Condition ;
      rdfs:comment "The provider of the data-cube is John Smith"^^xsd:string ;
      :hasDatacubeProvider
              :JohnSmith .

:Condition6
      rdf:type owl:NamedIndividual , :Condition ;
      rdfs:comment "The source of the data-cube is the lung cancer project study"^^xsd:string ;
	  :hasDimension l2s-dim:Dyslipidemia ;
      :hasDatacubeSource :LungCancerStudy .

:Condition7
      rdf:type owl:NamedIndividual , :Condition ;
      rdfs:comment "The project study has as sponsor the \"Xpharma\""^^xsd:string ;
	  :hasDimension l2s-dim:Dyslipidemia ;
      :hasDatacubeSource :LungCancerStudy .

:Condition8
      rdf:type owl:NamedIndividual , :Condition ;
      rdfs:comment "The project study is located in Greece"^^xsd:string ;
      :hasSPLocation "Greece"^^xsd:string .

:Condition9
      rdf:type owl:NamedIndividual , :Condition ;
      rdfs:comment "Gender is one of the dimensions of the cube" ;
      :hasDimension l2s-dim:Gender .

:DataProvider
      rdf:type owl:NamedIndividual , :Role .

:DateRange
      rdf:type owl:Class ;
      rdfs:subClassOf owl:Thing .

:DiabetesIncidences
      rdf:type owl:NamedIndividual , :Measure .

:Dimension
      rdf:type owl:Class ;
      rdfs:subClassOf owl:Thing .

:Drug
      rdf:type owl:NamedIndividual , :Dimension ;
      :hasDimesionValue "Aspirin"^^xsd:string .

:Dyslipidemia
      rdf:type owl:NamedIndividual , :Dimension .

:Gender
      rdf:type owl:NamedIndividual , :Dimension .

:JohnSmith
      rdf:type owl:NamedIndividual , :User ;
      :hasDisseminationPurpose
              "Publish in BIBE 2013"^^xsd:string ;
      :hasExpertise "Biologist"^^xsd:string ;
      :hasOccupation "Scientist"^^xsd:string ;
      :hasOrganization "CING"^^xsd:string ;
      :hasOrganizationType
              "ResearchInstitute"^^xsd:string ;
      :hasPurpose "Perform p-value analysis"^^xsd:string ;
      :hasQualification "PhD"^^xsd:string ;
      :hasRole :ClinicalTrialCoordinator ;
      :hasWorkingArea "Oncology"^^xsd:string .

:LungCancerStudy
      rdf:type owl:NamedIndividual , :StudyProject .

:MarySmith
      rdf:type owl:NamedIndividual , :User ;
      :hasLocation "Greece"^^xsd:string ;
      :hasPurpose "Perform p-value analysis "^^xsd:string ;
      :hasQualification "Student"^^xsd:string ;
      :hasRole :ClinicalResearcher ;
      :hasWorkingArea "Diabetes"^^xsd:string .

:Measure
      rdf:type owl:Class ;
      rdfs:subClassOf owl:Thing .

:NamedGraph
      rdf:type owl:Class ;
      rdfs:subClassOf rdfg-1:Graph .

:NamedGraph_11
      rdf:type :NamedGraph ;
      :hasGraphURI "http://www.linked2safety-project.eu/clinical-trials/dataset1/graph1"^^xsd:string ;
      :hasSparqlEndpoint "http://linked2safety.hcls.deri.org:3031/data-1/sparql"^^xsd:string .

:NamedGraph_12
      rdf:type :NamedGraph ;
      :hasGraphURI "http://www.linked2safety-project.eu/clinical-trials/dataset1/graph2"^^xsd:string ;
      :hasSparqlEndpoint "http://linked2safety.hcls.deri.org:3031/data-1/sparql"^^xsd:string .

:NamedGraph_13
      rdf:type :NamedGraph ;
      :hasGraphURI "http://www.linked2safety-project.eu/clinical-trials/dataset1/graph3"^^xsd:string ;
      :hasSparqlEndpoint "http://linked2safety.hcls.deri.org:3031/data-1/sparql"^^xsd:string .

:NamedGraph_14
      rdf:type :NamedGraph ;
      :hasGraphURI "http://www.linked2safety-project.eu/clinical-trials/dataset1/graph4"^^xsd:string ;
      :hasSparqlEndpoint "http://linked2safety.hcls.deri.org:3031/data-1/sparql"^^xsd:string .

:NamedGraph_15
      rdf:type :NamedGraph ;
      :hasGraphURI "http://www.linked2safety-project.eu/clinical-trials/dataset2/graph1"^^xsd:string ;
      :hasSparqlEndpoint "http://linked2safety.hcls.deri.org:3031/data-2/sparql"^^xsd:string .

:NamedGraph_16
      rdf:type :NamedGraph ;
      :hasGraphURI "http://www.linked2safety-project.eu/clinical-trials/dataset2/graph2"^^xsd:string ;
      :hasSparqlEndpoint "http://linked2safety.hcls.deri.org:3031/data-2/sparql"^^xsd:string .

:NamedGraph_17
      rdf:type :NamedGraph ;
      :hasGraphURI "http://www.linked2safety-project.eu/clinical-trials/dataset2/graph3"^^xsd:string ;
      :hasSparqlEndpoint "http://linked2safety.hcls.deri.org:3031/data-2/sparql"^^xsd:string .

:NamedGraph_18
      rdf:type :NamedGraph ;
      :hasGraphURI "http://www.linked2safety-project.eu/clinical-trials/dataset2/graph4"^^xsd:string ;
      :hasSparqlEndpoint "http://linked2safety.hcls.deri.org:3031/data-2/sparql"^^xsd:string .

:NamedGraph_19
      rdf:type :NamedGraph ;
      :hasGraphURI "http://www.linked2safety-project.eu/clinical-trials/dataset3/graph1"^^xsd:string ;
      :hasSparqlEndpoint "http://linked2safety.hcls.deri.org:3031/data-3/sparql"^^xsd:string .

:NamedGraph_20
      rdf:type :NamedGraph ;
      :hasGraphURI "http://www.linked2safety-project.eu/clinical-trials/dataset3/graph2"^^xsd:string ;
      :hasSparqlEndpoint "http://linked2safety.hcls.deri.org:3031/data-3/sparql"^^xsd:string .

:NamedGraph_21
      rdf:type :NamedGraph ;
      :hasGraphURI "http://www.linked2safety-project.eu/clinical-trials/dataset3/graph3"^^xsd:string ;
      :hasSparqlEndpoint "http://linked2safety.hcls.deri.org:3031/data-3/sparql"^^xsd:string .

:PlatformManager
      rdf:type owl:NamedIndividual , :Role .

:Role
      rdf:type owl:Class ;
      rdfs:subClassOf owl:Thing .

:StudyProject
      rdf:type owl:Class ;
      rdfs:subClassOf owl:Thing .

:User
      rdf:type owl:Class ;
      rdfs:subClassOf foaf:Agent .

:UserProfile
      rdf:type owl:Class ;
      rdfs:subClassOf owl:Thing .

:UserProfile_1
      rdf:type owl:NamedIndividual , :UserProfile ;
      rdfs:comment "The user profile refers to those users working in ZEINCRO" ;
      :hasOrganization "ZEINCRO"^^xsd:string .

:UserProfile_2
      rdf:type owl:NamedIndividual , :UserProfile ;
      rdfs:comment "The user profile refers to those users coming from Cyprus" ;
      :hasLocation "Cyprus"^^xsd:string .

:UserProfile_3
      rdf:type owl:NamedIndividual , :UserProfile ;
      rdfs:comment "The user profile refers to those users working in the area of oncology and coming from Cyprus"^^xsd:string ;
      :hasLocation "Greece"^^xsd:string ;
      :hasWorkingArea "Oncology"^^xsd:string .

:UserProfile_4
      rdf:type owl:NamedIndividual , :UserProfile ;
      rdfs:comment "The user profile refers to those users that has role 'ClinicalTrialCoordinator'"^^xsd:string ;
      :hasRole :ClinicalTrialCoordinator .

:appliesToNamedGraph
      rdf:type owl:ObjectProperty ;
      rdfs:comment "An access policy that applies to an lmds:NamedGraph. When an access policy has this property it means that the access policy applies to a NamedGraph (that contains a data-cube)."^^xsd:string ;
      rdfs:domain :AccessPolicy ;
      rdfs:range :NamedGraph .

:datacube-graph-2
      rdf:type owl:NamedIndividual , :NamedGraph ;
      rdfs:comment "The datacube-graph-2 represents a certain RDF data-cube that has four dimensions, namely sex, drug, snp and breast cancer"^^xsd:string .

:deniesAccess
      rdf:type owl:ObjectProperty ;
      rdfs:comment "The access control privilege which is not granted to the user. The access control is described using the Web Access Control vocabulary"^^xsd:string ;
      rdfs:domain :AccessPolicy ;
      rdfs:range acl:Read .

:grantsAccess
      rdf:type owl:ObjectProperty ;
      rdfs:comment "The access control privilege which is granted to the user. The access control is described using the Web Access Control vocabulary"^^xsd:string ;
      rdfs:domain :AccessPolicy ;
      rdfs:range acl:Read .

:hasCondition
      rdf:type owl:ObjectProperty ;
      rdfs:comment "The hasCondition defines the condition(s) (connected by 'and' logical operator when exceeds the one) that will be tested to specify the data-cubes restricted by the specific access policy"^^xsd:string ;
      rdfs:domain :AccessPolicy ;
      rdfs:range :Condition .

:hasDatacubeDate
      rdf:type owl:ObjectProperty ;
      rdfs:comment "The hasDatacubeDate property defines the date associated with the creation of the data cube"^^xsd:string ;
      rdfs:domain :Condition , :NamedGraph ;
      rdfs:range :DateRange .

:hasDatacubeDescription
      rdf:type owl:DatatypeProperty ;
      rdfs:comment "The hasDatacubeDescription property defines the description of the data cube" ;
      rdfs:domain :Condition , :NamedGraph ;
      rdfs:range xsd:string .

:hasDatacubeProvider
      rdf:type owl:ObjectProperty ;
      rdfs:comment "The DatacubeProvider defines the entity responsible for creating and making the data cube  available (or else the owner of the data cube)"^^xsd:string ;
      rdfs:domain :Condition , :NamedGraph ;
      rdfs:range :User .

:hasDatacubeSource
      rdf:type owl:ObjectProperty ;
      rdfs:comment "The DatacubeSource defines the source or else the study project from which the described data cube  has been derived"^^xsd:string ;
      rdfs:domain :Condition , :NamedGraph ;
      rdfs:range :StudyProject .

:hasDatacubeTitle
      rdf:type owl:DatatypeProperty ;
      rdfs:comment "The hasDatacubeTitle property defines the name/title of the data cube" ;
      rdfs:domain :Condition , :NamedGraph ;
      rdfs:range xsd:string .

:hasDimension
      rdf:type owl:ObjectProperty ;
      rdfs:comment "The hasDimension defines the dimension of the data-cube"^^xsd:string ;
      rdfs:domain :Condition , :NamedGraph ;
      rdfs:range :Dimension .

:hasDimesionValue
      rdf:type owl:DatatypeProperty ;
      rdfs:comment "The hasDimesionValue defines the value of a dimension based on which we will search for the data-cubes that are involved in a policy (e.g. if it's defined that Dimension Drug hasDimensionValue='aspirin', that means that we apply the specific policy to cubes having the Drug aspirin in their Dimensions' values)"^^xsd:string ;
      rdfs:domain :Dimension ;
      rdfs:range xsd:string .

:hasDisseminationPurpose
      rdf:type owl:DatatypeProperty ;
      rdfs:comment "The hasDisseminationPurpose property defines the dissemination purpose of the user from the results taken by the specific analysis of the data-cubes" ;
      rdfs:domain :User , :UserProfile ;
      rdfs:range xsd:string .

:hasEqualDate
      rdf:type owl:DatatypeProperty ;
      rdfs:comment "The hasEqualDate defines the exact date value "^^xsd:string ;
      rdfs:domain :DateRange ;
      rdfs:range xsd:date .

:hasEqualMeasureValue
      rdf:type owl:DatatypeProperty ;
      rdfs:comment "The hasEqualMeasureValue defines the the exact measure values based on which we will search for the data-cubes that are involved in a policy (e.g. if it's defined that Measure cases hasEqualMeasureValue=50, that means that we apply the specific policy to cubes having 50 cases in their Measures' values)"^^xsd:string ;
      rdfs:domain :Measure ;
      rdfs:range xsd:integer .

:hasExpertise
      rdf:type owl:DatatypeProperty ;
      rdfs:comment "e.g. biologist, epidemiologist, doctor"^^xsd:string ;
      rdfs:domain :User , :UserProfile ;
      rdfs:range xsd:string .

:hasGraphURI
      rdf:type owl:DatatypeProperty ;
      rdfs:domain :NamedGraph ;
      rdfs:range xsd:string .

:hasLocation
      rdf:type owl:DatatypeProperty ;
      rdfs:comment "The hasLocation property defines the location of the user" ;
      rdfs:domain :User , :UserProfile ;
      rdfs:range xsd:string .

:hasMaxDate
      rdf:type owl:DatatypeProperty ;
      rdfs:comment "The hasMaxDate defines the max date value "^^xsd:string ;
      rdfs:domain :DateRange ;
      rdfs:range xsd:date .

:hasMaxMeasureValue
      rdf:type owl:DatatypeProperty ;
      rdfs:comment "The hasMaxMeasureValue defines the the max measure values based on which we will search for the data-cubes that are involved in a policy (e.g. if it's defined that Measure cases hasMaxMeasureValue=50, that means that we apply the specific policy to cubes having until 50 cases in their Measures' values)"^^xsd:string ;
      rdfs:domain :Measure ;
      rdfs:range xsd:integer .

:hasMeasure
      rdf:type owl:ObjectProperty ;
      rdfs:comment "The hasMeasure defines the measured value of the phenomenon being observed"^^xsd:string ;
      rdfs:domain :Condition , :NamedGraph ;
      rdfs:range :Measure .

:hasMinDate
      rdf:type owl:DatatypeProperty ;
      rdfs:comment "The hasMinDate defines the min date value "^^xsd:string ;
      rdfs:domain :DateRange ;
      rdfs:range xsd:date .

:hasMinMeasureValue
      rdf:type owl:DatatypeProperty ;
      rdfs:comment "The hasMinMeasureValue defines the the max measure values based on which we will search for the data-cubes that are involved in a policy (e.g. if it's defined that Measure cases hasMinMeasureValue=50, that means that we apply the specific policy to cubes having more than 50 cases in their Measures' values)"^^xsd:string ;
      rdfs:domain :Measure ;
      rdfs:range xsd:integer .

:hasOccupation
      rdf:type owl:DatatypeProperty ;
      rdfs:comment "e.g. scientist, data analyst, etc."^^xsd:string ;
      rdfs:domain :User , :UserProfile ;
      rdfs:range xsd:string .

:hasOrganization
      rdf:type owl:DatatypeProperty ;
      rdfs:comment "The hasOrganization defines the organization for which the user is working"^^xsd:string ;
      rdfs:domain :User , :UserProfile ;
      rdfs:range xsd:string .

:hasOrganizationType
      rdf:type owl:DatatypeProperty ;
      rdfs:comment "e.g. a hospital, a clinical site, a pharmaceutical company, a CRO, an academic institute, a medical center, a genetic lab, a bioinformatics company, a health authority, etc."^^xsd:string ;
      rdfs:domain :User , :UserProfile ;
      rdfs:range xsd:string .

:hasPurpose
      rdf:type owl:DatatypeProperty ;
      rdfs:comment "The hasPurpose property defines the user’s purpose for sending the specific query"^^xsd:string ;
      rdfs:domain :User , :UserProfile ;
      rdfs:range xsd:string .

:hasQualification
      rdf:type owl:DatatypeProperty ;
      rdfs:comment "The hasQualification defines the education degree of the user e.g. Prof, PhD, MSc."^^xsd:string ;
      rdfs:domain :User , :UserProfile ;
      rdfs:range xsd:string .

:hasRole
      rdf:type owl:ObjectProperty ;
      rdfs:comment "The hasRole property defines the role of the user in the Linked2Safety system"^^xsd:string ;
      rdfs:domain :User , :UserProfile ;
      rdfs:range :Role .

:hasSPClinicaSite
      rdf:type owl:DatatypeProperty ;
      rdfs:comment "The SPClinicalSite defines the clinical sites/hospitals where the study project has been conducted"^^xsd:string ;
      rdfs:domain :Condition , :StudyProject ;
      rdfs:range xsd:string .

:hasSPDate
      rdf:type owl:ObjectProperty ;
      rdfs:comment "The hasSPDate property defines the point associated with the initialization of the study project"^^xsd:string ;
      rdfs:domain :Condition , :StudyProject ;
      rdfs:range :DateRange .

:hasSPDescription
      rdf:type owl:DatatypeProperty ;
      rdfs:comment "The hasSPDescription property defines the description of the study project"^^xsd:string ;
      rdfs:domain :Condition , :StudyProject ;
      rdfs:range xsd:string .

:hasSPLocation
      rdf:type owl:DatatypeProperty ;
      rdfs:comment "The hasSPLocation property defines the location/country of the clinical sites and hospitals where the study project has been conducted"^^xsd:string ;
      rdfs:domain :Condition , :StudyProject ;
      rdfs:range xsd:string .

:hasSPProvider
      rdf:type owl:ObjectProperty ;
      rdfs:comment "The SPProvider defines the entity responsible for running the study project"^^xsd:string ;
      rdfs:domain :Condition , :StudyProject ;
      rdfs:range :User .

:hasSPSponsor
      rdf:type owl:DatatypeProperty ;
      rdfs:comment "The SPSponsor defines the sponsor entity of the study project"^^xsd:string ;
      rdfs:domain :Condition , :StudyProject ;
      rdfs:range xsd:string .

:hasSPTitle
      rdf:type owl:DatatypeProperty ;
      rdfs:comment "The hasSPTitle property efines the name/title of the study project"^^xsd:string ;
      rdfs:domain :Condition , :StudyProject ;
      rdfs:range xsd:string .

:hasSparqlEndpoint
      rdf:type owl:DatatypeProperty ;
      rdfs:domain :NamedGraph ;
      rdfs:range xsd:string .

:hasSubscriptionDate
      rdf:type owl:ObjectProperty ;
      rdfs:comment "The hasSubscriptionDate property defines the subscription date of the user in the system"^^xsd:string ;
      rdfs:domain :User , :UserProfile ;
      rdfs:range :DateRange .

:hasUser
      rdf:type owl:ObjectProperty ;
      rdfs:comment "The hasUser defines the user who is granted or denied the specific access policy "^^xsd:string ;
      rdfs:domain :AccessPolicy ;
      rdfs:range :User .

:hasUserProfile
      rdf:type owl:ObjectProperty ;
      rdfs:comment "The hasUserProfile defines a set of attributes (i.e. a pattern/profile) that the requester user must satisfy to be authorized to read the specific data-cube"^^xsd:string ;
      rdfs:domain :AccessPolicy ;
      rdfs:range :UserProfile .

:hasWorkingArea
      rdf:type owl:DatatypeProperty ;
      rdfs:comment "The hasWorkingArea property defines the subject area of the user’s job"^^xsd:string ;
      rdfs:domain :UserProfile ;
      rdfs:domain
              [ rdf:type owl:Class ;
                owl:unionOf (:User :UserProfile)
              ] ;
      rdfs:range xsd:string .

rdfs:Class
      rdf:type owl:Class .

xsd:date
      rdf:type rdfs:Datatype .

rdfg-1:Graph
      rdf:type owl:Class ;
      rdfs:comment """
An RDF graph (with intensional semantics).
      """ ;
      rdfs:label "Graph" .

rdfg-1:equivalentGraph
      rdf:type owl:AnnotationProperty , owl:ObjectProperty ;
      rdfs:comment """
The graphs associated with the subject and object are equivalent.
      """ ;
      rdfs:domain rdfg-1:Graph ;
      rdfs:range rdfg-1:Graph .

rdfg-1:subGraphOf
      rdf:type owl:AnnotationProperty , owl:ObjectProperty ;
      rdfs:comment """
The graph associated with the subject is a subgraph of a graph equivalent
to that associated with the object.
      """ ;
      rdfs:domain rdfg-1:Graph ;
      rdfs:range rdfg-1:Graph .

ont:InformationResource
      rdf:type owl:Class .

<http://www.w3.org/ns/auth/acl>
      rdfs:comment """Defines the element of Authorization and its essential properties,
    and also some classes of access such as read and write. """ ;
      dc:title "Basic Access Control ontology" .

acl:Access
      rdf:type owl:Class ;
      rdfs:comment "Any kind of access to a resource. Don't use this, use R W and RW" ;
      acl:label "access"@en .

acl:Append
      rdf:type owl:Class ;
      rdfs:comment """Append accesses are specific write access which only add information, and do not remove information.
    For text files, for example, append access allows bytes to be added onto the end of the file.
    For RDF graphs, Append access allows adds triples to the graph but does not remove any.
    Append access is useful for dropbox functionality.
    Dropbox can be used for link notification, which the information added is a notification
    that a some link has been made elsewhere relevant to the given resource.
    """ ;
      rdfs:label "append"@en ;
      rdfs:subClassOf acl:Access , acl:Write .

acl:Authorization
      rdf:type owl:Class ;
      rdfs:comment """An element of access control,
    allowing agent to agents access of some kind to resources or classes of resources""" ;
      rdfs:label "authorization" .

acl:Control
      rdf:type owl:Class ;
      rdfs:comment "Allows read/write access to the ACL for the resource(s)" ;
      rdfs:label "control"@en ;
      rdfs:subClassOf acl:Access .

acl:Read
      rdf:type owl:Class ;
      rdfs:comment "The class of read operations" ;
      rdfs:label "read"@en ;
      rdfs:subClassOf acl:Access .

acl:Read_l2s
      rdf:type acl:Read , owl:NamedIndividual .

acl:Write
      rdf:type owl:Class ;
      rdfs:label "write"@en ;
      rdfs:subClassOf acl:Access .

acl:accessControl
      rdf:type owl:AnnotationProperty ;
      rdfs:comment """The Access Control file for this information resource.
        This may of course be a virtual resorce implemented by the access control system.
        Note also HTTP's header  Link:  foo.meta ;rel=meta can be used for this.""" ;
      rdfs:domain ont:InformationResource ;
      rdfs:label "access control" ;
      rdfs:range ont:InformationResource ;
      rdfs:subPropertyOf rdfs:seeAlso .

acl:accessTo
      rdf:type owl:AnnotationProperty , owl:ObjectProperty ;
      rdfs:comment "The information resource to which access is being granted." ;
      rdfs:domain acl:Authorization ;
      rdfs:range ont:InformationResource .

acl:accessToClass
      rdf:type owl:AnnotationProperty , owl:ObjectProperty ;
      rdfs:comment "A class of information resources to which access is being granted." ;
      rdfs:domain acl:Authorization ;
      rdfs:range rdfs:Class .

acl:agent
      rdf:type owl:AnnotationProperty , owl:ObjectProperty ;
      rdfs:comment "A person or social entity to being given the right" ;
      rdfs:domain acl:Authorization ;
      rdfs:range foaf:Agent .

acl:agentClass
      rdf:type owl:AnnotationProperty , owl:ObjectProperty ;
      rdfs:comment "A class of persons or social entities to being given the right" ;
      rdfs:domain acl:Authorization ;
      rdfs:range rdfs:Class .

acl:defaultForNew
      rdf:type owl:AnnotationProperty ;
      rdfs:comment "A directory for which this authorization is used for new files in the directory." ;
      rdfs:domain acl:Authorization ;
      rdfs:label "default access for new things in" .

acl:label
      rdf:type owl:AnnotationProperty .

acl:mode
      rdf:type owl:AnnotationProperty , owl:ObjectProperty ;
      rdfs:comment "A mode of access such as read or write." ;
      rdfs:domain acl:Authorization ;
      rdfs:range rdfs:Class .

acl:owner
      rdf:type owl:ObjectProperty ;
      rdfs:comment """The person or other agent which owns this. 
    For example, the owner of a file in a filesystem.
    There is a sense of right to control.   Typically defaults to the agent who craeted
    something but can be changed.""" ;
      rdfs:range foaf:Agent .

foaf:Agent
      rdf:type owl:Class .
